Lean4Lean/Verify/Environment/Lemmas.lean
@@ -5,6 +5,10 @@ namespace Lean4Lean
 open Lean hiding Environment Exception
 open Kernel
 
+theorem TrConstant.sf_mono (hsf : safety ≤ safety')
+    (H : TrConstant safety' env ci ci') : TrConstant safety env ci ci' :=
+  ⟨safety.le_trans hsf H.1, H.2⟩
+
 theorem TrConstant.mono {env env' : VEnv} (henv : env ≤ env')
     (H : TrConstant safety env ci ci') : TrConstant safety env' ci ci' :=
   ⟨H.1, H.2.1, H.2.2.mono henv⟩
@@ -17,38 +21,40 @@ theorem TrDefVal.mono {env env' : VEnv} (henv : env ≤ env')
     (H : TrDefVal safety env ci ci') : TrDefVal safety env' ci ci' :=
   ⟨H.1.mono henv, H.2.mono henv⟩
 
-variable (safety : DefinitionSafety) (env : VEnv) in
-inductive Aligned1 : ConstantInfo → Option VConstant → Prop where
-  | block : ¬isAsSafeAs safety ci → Aligned1 ci none
-  | const : TrConstant safety env ci ci' → Aligned1 ci (some ci')
-
 variable (safety : DefinitionSafety) in
 inductive Aligned : ConstMap → VEnv → Prop where
   | empty : Aligned {} .empty
-  | const : Aligned C venv → Aligned1 safety venv ci ci' →
+  | ignoreConst : Aligned C venv → C.find? n = none → ¬safety ≤ ci.safety →
+    ci.name = n → Aligned (C.insert n ci) venv
+  | const : Aligned C venv → C.find? n = none → TrConstant safety venv ci ci' →
     venv.addConst n ci' = some venv' → ci.name = n → Aligned (C.insert n ci) venv'
   | defeq : Aligned C venv → Aligned C (venv.addDefEq df)
 
-theorem Aligned.map_wf' (H : Aligned safety C venv) :
-    C.WF ∧ ∀ n, (C.find? n).isSome = (venv.constants n).isSome := by
+theorem Aligned.map_wf (H : Aligned safety C venv) : C.WF := by
   induction H with
-  | empty => exact ⟨.empty, by simp [SMap.find?, VEnv.empty]⟩
-  | @const _ _ _ _ n _ _ _ eq _ ih =>
-    simp [VEnv.addConst] at eq; split at eq <;> cases eq
-    have := ih.2 n; simp_all [-ih]
-    refine ⟨.insert ih.1 _ _ this, fun n' => ?_⟩
-    simp [ih.1.find?_insert]; split <;> simp [ih.2]
+  | empty => exact .empty
+  | ignoreConst _ h1 _ _ ih
+  | const _ h1 _ _ _ ih => exact ih.insert _ _ h1
   | defeq _ ih => exact ih
 
-theorem Aligned.map_wf (H : Aligned safety C venv) : C.WF := H.map_wf'.1
-theorem Aligned.find?_isSome (H : Aligned safety C venv) :
-    (C.find? n).isSome = (venv.constants n).isSome := H.map_wf'.2 _
+theorem Aligned.find?_iff (H : Aligned safety C venv) :
+    (∃ ci, C.find? name = some ci ∧ safety ≤ ci.safety) ↔ ∃ ci, venv.constants name = some ci := by
+  induction H with
+  | empty => simp [SMap.find?, VEnv.empty]
+  | ignoreConst H _ h2 _ ih =>
+    simp [H.map_wf.find?_insert]; split <;> [skip; assumption]
+    rename_i eq1 eq2; subst eq2; simp [← ih, *]
+  | const H h1 h2 eq _ ih =>
+    simp [H.map_wf.find?_insert]
+    simp [VEnv.addConst] at eq; split at eq <;> cases eq
+    split <;> simp_all; exact h2.1
+  | defeq _ ih => exact ih
 
 theorem Aligned.addQuot1 {Q : Prop}
     (H1 : ∀ c env, Aligned safety c env → P c env → Q)
     (C env) (wf : Aligned safety C env) (H2 : AddQuot1 n k ci P C env) : Q := by
-  let ⟨_, _, h1, h2, h3, h4⟩ := H2
-  exact H1 _ _ (wf.const (.const ⟨by cases safety <;> rfl, h2.2⟩) h3 rfl) h4
+  let ⟨_, _, _, h1, h2, h3, h4⟩ := H2
+  exact H1 _ _ (wf.const h2 (h1.sf_mono DefinitionSafety.le_safe) h3 rfl) h4
 
 nonrec theorem Aligned.addQuot (H : AddQuot C₁ C₂ venv₁ venv₂)
     (wf : Aligned safety C₁ venv₁) : Aligned safety C₂ venv₂ := by
@@ -63,65 +69,76 @@ theorem Aligned.addInduct (H : AddInduct C₁ venv₁ decl C₂ venv₂) :
 theorem TrEnv'.aligned (H : TrEnv' safety C Q venv) : Aligned safety C venv := by
   induction H with
   | empty => exact .empty
-  | block hs h _ ih => exact ih.const (.block hs) h rfl
-  | «axiom» h1 _ h _ ih => exact ih.const (.const h1) h rfl
-  | «opaque» h1 _ h _ ih => exact ih.const (.const h1.1.1) h rfl
-  | defn h1 _ h _ ih => exact (ih.const (.const h1.1.1) h rfl).defeq
+  | «axiom» h1 h2 _ h _ ih => exact ih.const h2 h1 h rfl
+  | «opaque» h1 h2 _ h _ ih => exact ih.const h2 h1.1.1 h rfl
+  | defn h1 h2 _ h _ ih => exact (ih.const h2 h1.1.1 h rfl).defeq
   | quot _ h _ ih => exact ih.addQuot h
   | induct _ h _ ih => exact ih.addInduct h
 
 theorem TrEnv'.map_wf (H : TrEnv' safety C Q venv) : C.WF := H.aligned.map_wf
 
 theorem Aligned.find? (H : Aligned safety C venv)
-    (h : C.find? name = some ci) (hs : isAsSafeAs safety ci) :
-    ∃ ci', venv.constants name = some (some ci') ∧ TrConstant safety venv ci ci' := by
+    (h : C.find? name = some ci) (hs : safety ≤ ci.safety) :
+    ∃ ci', venv.constants name = some ci' ∧ TrConstant safety venv ci ci' := by
   have mono {env₁ env₂} (H : env₁.LE env₂) :
-      (∃ ci', env₁.constants name = some (some ci') ∧ TrConstant safety env₁ ci ci') →
-      (∃ ci', env₂.constants name = some (some ci') ∧ TrConstant safety env₂ ci ci')
+      (∃ ci', env₁.constants name = some ci' ∧ TrConstant safety env₁ ci ci') →
+      (∃ ci', env₂.constants name = some ci' ∧ TrConstant safety env₂ ci ci')
     | ⟨_, h1, h2⟩ => ⟨_, H.constants h1, h2.mono H⟩
   induction H with
   | empty => simp [SMap.find?] at h
-  | const h1 h2 h3 h4 ih =>
+  | ignoreConst h1 _ _ _ ih =>
+    rw [h1.map_wf.find?_insert] at h; split at h
+    · cases h; contradiction
+    · exact ih h
+  | const h1 _ h2 h3 _ ih =>
     have := VEnv.addConst_le h3
     rw [h1.map_wf.find?_insert] at h; split at h
-    · cases h; rename_i n _ h; simp at h; subst n h
+    · rename_i h'; cases h; simp at h'; subst h'
       simp [VEnv.addConst] at h3; split at h3 <;> cases h3
-      cases h2; · contradiction
-      simp; rename_i h'; exact h'.mono this
+      simp; rename_i h'; refine h2.mono this
     · let ⟨_, h1, h2⟩ := ih h; exact ⟨_, this.constants h1, h2.mono this⟩
   | defeq h1 ih => let ⟨_, h1, h2⟩ := ih h; exact ⟨_, h1, h2.mono VEnv.addDefEq_le⟩
 
 theorem Aligned.find?_uniq (H : Aligned safety C venv)
-    (h : C.find? name = some ci) (hs : venv.constants name = some (some ci')) :
+    (h : C.find? name = some ci) (hs : venv.constants name = some ci') :
     ci.name = name ∧ TrConstant safety venv ci ci' := by
   induction H with
   | empty => simp [SMap.find?] at h
-  | const h1 h2 h3 h4 ih =>
+  | ignoreConst H h2 h3 _ ih =>
+    simp [H.map_wf.find?_insert] at h; split at h
+    · rename_i n ci _ h'; subst n h'
+      simpa [h2, hs] using H.find?_iff (name := ci.name)
+    · exact ih h hs
+  | const h1 h5 h2 h3 h4 ih =>
     have := VEnv.addConst_le h3
     simp [VEnv.addConst] at h3; split at h3 <;> cases h3
     simp [h1.map_wf.find?_insert] at h hs; revert h hs; split
-    · rintro ⟨⟩ ⟨⟩; rename_i n _ _ _; subst n
-      let .const h2 := h2; exact ⟨h4, h2.mono this⟩
+    · rintro ⟨⟩ ⟨⟩; rename_i n _ _ _; subst n; exact ⟨h4, h2.mono this⟩
     · intro hs h; let ⟨h1, h2⟩ := ih h hs; exact ⟨h1, h2.mono this⟩
   | defeq h1 ih => let ⟨h1, h2⟩ := ih h hs; exact ⟨h1, h2.mono VEnv.addDefEq_le⟩
 
 theorem TrEnv.find?_iff (H : TrEnv safety env venv) :
-    (∃ ci, env.find? name = some ci) ↔ ∃ oci, venv.constants name = some oci := by
-  conv => enter [1,1,_,1]; apply H.map_wf.find?'_eq_find?
-  erw [← Option.isSome_iff_exists, H.aligned.find?_isSome, Option.isSome_iff_exists]
+    (∃ ci, env.find? name = some ci ∧ safety ≤ ci.safety) ↔ ∃ ci, venv.constants name = some ci := by
+  conv => enter [1,1,_,1,1]; apply H.map_wf.find?'_eq_find?
+  exact H.aligned.find?_iff
+
+-- theorem TrEnv.contains_iff (H : TrEnv safety env venv) :
+--     env.contains name ↔ ∃ oci, venv.constants name = some oci := by
+--   simp [← H.find?_iff, Kernel.Environment.find?, H.map_wf.find?'_eq_find?,
+--     ← Option.isSome_iff_exists, ← SMap.find?_isSome, Kernel.Environment.contains]
 
 theorem TrEnv.find? (H : TrEnv safety env venv)
-    (h : env.find? name = some ci) (hs : isAsSafeAs safety ci) :
-    ∃ ci', venv.constants name = some (some ci') ∧ TrConstant safety venv ci ci' :=
+    (h : env.find? name = some ci) (hs : safety ≤ ci.safety) :
+    ∃ ci', venv.constants name = some ci' ∧ TrConstant safety venv ci ci' :=
   H.aligned.find? (H.map_wf.find?'_eq_find? _ ▸ h) hs
 
 theorem TrEnv.find?_uniq (H : TrEnv safety env venv)
-    (h : env.find? name = some ci) (hs : venv.constants name = some (some ci')) :
+    (h : env.find? name = some ci) (hs : venv.constants name = some ci') :
     ci.name = name ∧ TrConstant safety venv ci ci' :=
   H.aligned.find?_uniq (H.map_wf.find?'_eq_find? _ ▸ h) hs
 
 theorem TrEnv'.of_value (H : TrEnv' safety C Q venv) (h : C.find? name = some ci)
-    (hs : isAsSafeAs safety ci) (hv : ci.value? = some v) :
+    (hs : safety ≤ ci.safety) (hv : ci.value? = some v) :
     TrExpr venv ci.levelParams [] v (.const ci.name (VLevel.params ci.levelParams.length)) := by
   have {C n ci'} (hC : C.WF) :
       (SMap.insert C n ci').find? name = some ci →
@@ -129,17 +146,17 @@ theorem TrEnv'.of_value (H : TrEnv' safety C Q venv) (h : C.find? name = some ci
     rw [hC.find?_insert]; simp; split <;> simp +contextual [*]
   induction H with
   | empty => simp [SMap.find?] at h
-  | block _ h1 H ih | «axiom» _ _ h1 H ih | «opaque» _ _ h1 H ih =>
+  | «axiom» _ _ _ h1 H ih | «opaque» _ _ _ h1 H ih =>
     obtain h | ⟨rfl, rfl⟩ := this H.map_wf h
     · exact (ih h).mono (VEnv.addConst_le h1)
     · contradiction
-  | defn h2 h3 h1 H ih =>
+  | defn h2 h3 h4 h1 H ih =>
     have' le := (VEnv.addConst_le h1).trans VEnv.addDefEq_le
     obtain h | ⟨rfl, rfl⟩ := this H.map_wf h
     · exact (ih h).mono le
     · cases hv
       have := VEnv.IsDefEq.extra0 VEnv.addDefEq_self <|
-        (H.defn h2 h3 h1).wf.ordered.defEqWF VEnv.addDefEq_self
+        (H.defn h2 h3 h4 h1).wf.ordered.defEqWF VEnv.addDefEq_self
       let ⟨⟨⟨b1, b2, b3⟩, b4⟩, b5⟩ := h2
       refine ⟨_, b5.mono le, b2.symm ▸ b4.symm ▸ ⟨_, this.symm⟩⟩
   | quot _ h1 H ih =>
@@ -147,14 +164,14 @@ theorem TrEnv'.of_value (H : TrEnv' safety C Q venv) (h : C.find? name = some ci
         ∀ C env, Aligned safety C env → AddQuot1 n k ci' P C env → C.find? name = some ci by
       refine (ih <| this (this <| this <| this ?_) _ _ H.aligned h1).mono h1.le
       rintro _ _ _ ⟨rfl, rfl⟩; exact h
-    rintro n k ci' P ih C env wf ⟨_, h1, _, h2, h3, h4⟩
-    have wf' := wf.const (.const ⟨by cases safety <;> rfl, h2.2⟩) h3 rfl
-    obtain h | ⟨rfl, rfl⟩ := this wf.map_wf (ih _ _ wf' h4)
+    rintro n k ci' P ih C env wf ⟨_, h1, _, h2, h3, h4, h5⟩
+    have wf' := wf.const h3 ⟨by cases safety <;> rfl, h2.2⟩ h4 rfl
+    obtain h | ⟨rfl, rfl⟩ := this wf.map_wf (ih _ _ wf' h5)
     · exact h
     · contradiction
   | induct _ h1 H ih => cases h1
 
 nonrec theorem TrEnv.of_value (H : TrEnv safety env venv) (h : env.find? name = some ci)
-    (hs : isAsSafeAs safety ci) (hv : ci.value? = some v) :
+    (hs : safety ≤ ci.safety) (hv : ci.value? = some v) :
     TrExpr venv ci.levelParams [] v (.const ci.name (VLevel.params ci.levelParams.length)) :=
   H.of_value (by rwa [← H.map_wf.find?'_eq_find?]) hs hv
