Lean4Lean/Theory/Typing/EnvLemmas.lean
@@ -11,15 +11,14 @@ theorem VEnv.WF.ordered : WF env → Ordered env
     | empty => exact .empty
     | decl h _ ih =>
       cases h with
-      | block h => exact .const ih (by rintro _ ⟨⟩) h
-      | «axiom» h1 h2 => exact .const ih (by rintro _ ⟨⟩; exact h1) h2
+      | «axiom» h1 h2 => exact .const ih h1 h2
       | @«def» env env' ci h1 h2 =>
-        refine .defeq (.const ih (by rintro _ ⟨⟩; exact h1.isType ih ⟨⟩) h2) ⟨?_, ?_⟩
+        refine .defeq (.const ih (h1.isType ih ⟨⟩) h2) ⟨?_, ?_⟩
         · simp [VDefVal.toDefEq]
           rw [← (h1.levelWF ⟨⟩).2.2.instL_id]
           exact .const (addConst_self h2) VLevel.id_WF (by simp)
         · exact h1.mono (addConst_le h2)
-      | «opaque» h1 h2 => exact .const ih (by rintro _ ⟨⟩; exact h1.isType ih ⟨⟩) h2
+      | «opaque» h1 h2 => exact .const ih (h1.isType ih ⟨⟩) h2
       | «example» _ => exact ih
       | quot h1 h2 => exact addQuot_WF ih h1 h2
       | induct h1 h2 => exact addInduct_WF ih h1 h2
