Lean4Lean/Theory/Typing/Meta.lean
@@ -7,11 +7,11 @@ theorem with_addConst {P : Prop} {env env' : VEnv} {cis : List VObject}
     (henv : Ordered env)
     (hci : env.HasObjects cis → ci.WF env)
     (IH : ∀ {env1}, Ordered env1 →
-      env1.HasObjects (.const n (some ci) :: cis) → f env1 = some env' → P)
+      env1.HasObjects (.const n ci :: cis) → f env1 = some env' → P)
     (hcis : env.HasObjects cis)
-    (H : (env.addConst n (some ci) >>= f) = some env') : P := by
+    (H : (env.addConst n ci >>= f) = some env') : P := by
   let ⟨env1, h1, henv1⟩ := Option.bind_eq_some_iff.1 H
-  refine IH (.const henv (by rintro _ ⟨⟩; exact hci hcis) h1) (hcis.const h1) henv1
+  refine IH (.const henv (hci hcis) h1) (hcis.const h1) henv1
 
 theorem Lookup.zero' (eq : A.lift = ty') :
     Lookup (A::Γ) 0 ty' := eq ▸ .zero
@@ -28,7 +28,7 @@ macro_rules | `(tactic| lookup_tac) => `(tactic|
 theorem HasType.app' (h1 : HasType env U Γ f (.forallE A B)) (h2 : HasType env U Γ a A)
     (eq : B.inst a = B') : HasType env U Γ (.app f a) B' := eq ▸ .appDF h1 h2
 theorem HasType.const'
-  (h1 : constants env c = some (some ci))
+  (h1 : constants env c = some ci)
   (h2 : ∀ (l : VLevel), l ∈ ls → VLevel.WF uvars l)
   (h3 : List.length ls = ci.uvars)
   (eq : .instL ls ci.type = ty') :
